pcuic/theories/PCUICGlobalEnv.v
@@ -1,0 +1,77 @@
+(* Distributed under the terms of the MIT license. *)
+From Coq Require Import ProofIrrelevance.
+From MetaCoq.Template Require Import config utils uGraph.
+From MetaCoq.PCUIC Require Import PCUICAst PCUICAstUtils
+     PCUICReflect PCUICTyping.
+
+Definition wf_global_uctx_invariants {cf:checker_flags} Σ :
+  wf Σ ->
+  global_uctx_invariants (global_uctx Σ).
+Proof.
+ intros HΣ. split.
+ - cbn. eapply LevelSet.mem_spec, global_levels_Set.
+ - unfold global_uctx.
+   simpl. intros [[l ct] l'] Hctr. simpl in *.
+   induction Σ in HΣ, l, ct, l', Hctr |- *.
+   + apply ConstraintSetFact.empty_iff in Hctr; contradiction.
+   + simpl in *. apply ConstraintSet.union_spec in Hctr.
+     destruct Hctr as [Hctr|Hctr].
+     * split.
+       -- inversion HΣ; subst.
+          destruct H2 as [HH1 [HH HH3]].
+          subst udecl. destruct d as [decl|decl]; simpl in *.
+          ++ destruct decl; simpl in *.
+             destruct cst_universes ; [
+               eapply (HH (l, ct, l') Hctr)
+             | apply ConstraintSetFact.empty_iff in Hctr ; contradiction
+             ].
+          ++ destruct decl. simpl in *.
+             destruct ind_universes ; [
+               eapply (HH (l, ct, l') Hctr)
+             | apply ConstraintSetFact.empty_iff in Hctr; contradiction
+             ].
+       -- inversion HΣ. subst.
+          destruct H2 as [HH1 [HH HH3]].
+          subst udecl. destruct d as [decl|decl].
+          all: simpl in *.
+          ++ destruct decl. simpl in *.
+             destruct cst_universes ; [
+               eapply (HH (l, ct, l') Hctr)
+             | apply ConstraintSetFact.empty_iff in Hctr; contradiction
+             ].
+          ++ destruct decl. simpl in *.
+             destruct ind_universes; [
+               eapply (HH (l, ct, l') Hctr)
+             | apply ConstraintSetFact.empty_iff in Hctr; contradiction
+             ].
+     * inversion HΣ. subst.
+       split.
+       all: apply LevelSet.union_spec.
+       all: right.
+       all: unshelve eapply (IHΣ _ _ _ _ Hctr).
+       all: try eassumption.
+Qed.
+
+Definition wf_ext_global_uctx_invariants {cf:checker_flags} Σ :
+  wf_ext Σ ->
+  global_uctx_invariants (global_ext_uctx Σ).
+Proof.
+ intros HΣ. split.
+ - apply LevelSet.union_spec. right. apply LevelSet.mem_spec, global_levels_Set.
+ - destruct Σ as [Σ φ]. destruct HΣ as [HΣ Hφ].
+   destruct (wf_global_uctx_invariants _ HΣ) as [_ XX].
+   unfold global_ext_uctx, global_ext_levels, global_ext_constraints.
+   simpl. intros [[l ct] l'] Hctr. simpl in *. apply ConstraintSet.union_spec in Hctr.
+   destruct Hctr as [Hctr|Hctr].
+   + destruct Hφ as [_ [HH _]]. apply (HH _ Hctr).
+   + specialize (XX _ Hctr).
+     split; apply LevelSet.union_spec; right; apply XX.
+Qed.
+
+Definition global_ext_uctx_consistent {cf:checker_flags} Σ
+ : wf_ext Σ -> consistent (global_ext_uctx Σ).2.
+Proof. 
+  intros HΣ. cbn. unfold global_ext_constraints.
+  unfold wf_ext, on_global_env_ext in HΣ.
+  destruct HΣ as [_ [_ [_ HH]]]. apply HH.
+Qed.
